Core/Util.lean
@@ -84,29 +84,29 @@ theorem Ren.add_one_commutes [RenMap T] [SubstMap T T] [SubstMapId T T] {y : Nat
   funext; case _ x =>
   simp [Ren.to, Subst.compose]; omega
 
-def List.rmap [i : RenMap S] (lf : Endo Ren) (r : Ren) : List S -> List S
+def List.rmap [i : RenMap S] (r : Ren) : List S -> List S
 | [] => []
-| .cons x tl => (i.rmap lf r x) :: rmap lf r tl
+| .cons x tl => (i.rmap r x) :: rmap r tl
 
 instance [RenMap S] : RenMap (List S) where
   rmap := List.rmap
 
-def List.smap [RenMap T] [SubstMap S T] (lf : Endo (Subst T)) (σ : Subst T) : List S -> List S
+def List.smap [RenMap T] [SubstMap S T] (σ : Subst T) : List S -> List S
 | [] => []
-| .cons x tl => x[σ:_] :: smap lf σ tl
+| .cons x tl => x[σ:_] :: smap σ tl
 
 instance SubstMap_List  [RenMap T] [SubstMap S T] : SubstMap (List S) T where
   smap := List.smap
 
 @[simp]
 theorem List.smap_nil [RenMap T] [SubstMap S T] {σ : Subst T} : (@List.nil S)[σ:_] = [] := by
-  simp [Subst.apply, SubstMap.smap, List.smap]
+  simp [SubstMap.smap, List.smap]
 
 @[simp]
 theorem List.smap_cons [RenMap T] [SubstMap S T] {x} {tl : List S} {σ : Subst T}
   : (x :: tl)[σ:_] = x[σ:_] :: tl[σ:_]
 := by
-  simp [Subst.apply, SubstMap.smap, List.smap]
+  simp [SubstMap.smap, List.smap]
 
 instance [RenMap T] [SubstMap S T] [SubstMapId S T]
   : SubstMapId (List S) T
