Core/Vec.lean
@@ -1,369 +1,327 @@
 import LeanSubst
+import Lilac.Vect
 
 open LeanSubst
+open Vect
 
-def Fin.cases1
-  {motive : Fin 1 -> Prop}
-  (h : motive 0)
-  (v : Fin 1) : motive v
-:= by
-  induction v using Fin.induction; simp [*]
-  case _ i _ => apply Fin.elim0 i
+protected def Vect.reprPrec [Repr T] : {n : Nat} -> Vect n T -> Nat -> Std.Format
+| 0, _, _ => ""
+| 1, v, _ => repr (v 0)
+| n + 1, v, i =>
+  let ⟨h , t⟩ := v.uncons
+  (repr h) ++ ", " ++ (Vect.reprPrec t i)
 
-def Fin.cases2
-  {motive : Fin 2 -> Prop}
-  (h1 : motive 0) (h2 : motive 1)
-  (v : Fin 2) : motive v
-:= by
-  induction v using Fin.induction; simp [*]
-  case _ i h =>
-    induction i using Fin.induction; simp [*]
-    case _ i h => apply Fin.elim0 i
-
-def Vec (T : Sort u) (n : Nat) := Fin n -> T
-
-def Vec.nil : Vec T 0 := λ x => nomatch x
-
-def Vec.cons (t : T) (xs : Vec T n) : Vec T (n + 1)
-| n => if h : n = 0 then t else xs (Fin.pred n h)
-
-infixr:55 "::" => Vec.cons
-
-def Vec.drop : Vec T (n + 1) -> Vec T n
-| v => λ i => v (Fin.succ i)
-
-def Vec.uncons :  Vec T (n + 1) -> T × Vec T n
-| v => (v 0, drop v)
-
-
-protected def Vec.reprPrec [Repr T] : {n : Nat} -> Vec T n -> Nat -> Std.Format
+protected def Vect.reprPrec' (repr : T -> Std.Format) : {n : Nat} -> Vect n T -> Nat -> Std.Format
 | 0, _, _ => ""
 | 1, v, _ => repr (v 0)
 | _ + 1, v, i =>
-  let (h, t) := uncons v
-  (repr h) ++ ", " ++ (Vec.reprPrec t i)
-
-protected def Vec.reprPrec' (repr : T -> Std.Format) : {n : Nat} -> Vec T n -> Nat -> Std.Format
-| 0, _, _ => ""
-| 1, v, _ => repr (v 0)
-| _ + 1, v, i =>
-  let (h, t) := uncons v
-  (repr h) ++ ", " ++ (Vec.reprPrec' repr t i)
+  let ⟨h, t⟩ := uncons v
+  (repr h) ++ ", " ++ (Vect.reprPrec' repr t i)
 
 
-instance [Repr T] : Repr (Vec T n) where
-  reprPrec v n := "v[" ++ Vec.reprPrec v n ++ "]"
+instance [Repr T] : Repr (Vect n T) where
+  reprPrec v n := "v[" ++ Vect.reprPrec v n ++ "]"
 
-syntax "v[" withoutPosition(term,*,?) "]"  : term
+-- syntax "v[" withoutPosition(term,*,?) "]"  : term
 
--- Adapted from Lean Prelude
-macro_rules
-| `(v[ $elems,* ]) => do
-  let rec expandVecList (i : Nat) (result : Lean.TSyntax `term) : Lean.MacroM Lean.Syntax := do
-    match i with
-    | 0 => pure result
-    | i + 1 => expandVecList i (<- ``(Vec.cons `$(⟨elems.getElems.get!Internal i⟩) $result))
-  let size := elems.getElems.size
-  expandVecList size (<- ``(Vec.nil))
+-- -- Adapted from Lean Prelude
+-- macro_rules
+-- | `(v[ $elems,* ]) => do
+--   let rec expandVectList (i : Nat) (result : Lean.TSyntax `term) : Lean.MacroM Lean.Syntax := do
+--     match i with
+--     | 0 => pure result
+--     | i + 1 => expandVectList i (<- ``(Vect.cons `$(⟨elems.getElems.get!Internal i⟩) $result))
+--   let size := elems.getElems.size
+--   expandVectList size (<- ``(Vect.nil))
 
--- Adapted from Lean Prelude
-@[app_unexpander Vec.nil]
-meta def unexpandVecNil : Lean.PrettyPrinter.Unexpander
-| `($(_)) => `(v[])
+-- -- Adapted from Lean Prelude
+-- @[app_unexpander Vect.nil]
+-- meta def unexpandVectNil : Lean.PrettyPrinter.Unexpander
+-- | `($(_)) => `(v[])
 
--- Adapted from Lean Prelude
-@[app_unexpander Vec.cons]
-meta def unexpandVecCons : Lean.PrettyPrinter.Unexpander
-| `($(_) $x $tail) =>
-  match tail with
-  | `(v[])      => `(v[$x])
-  | `(v[$xs,*]) => `(v[$x, $xs,*])
-  | `(⋯)       => `(v[$x, $tail]) -- Unexpands to `[x, y, z, ⋯]` for `⋯ : List α`
-  | _          => throw ()
-| _ => throw ()
+-- -- Adapted from Lean Prelude
+-- @[app_unexpander Vect.cons]
+-- meta def unexpandVectCons : Lean.PrettyPrinter.Unexpander
+-- | `($(_) $x $tail) =>
+--   match tail with
+--   | `(v[])      => `(v[$x])
+--   | `(v[$xs,*]) => `(v[$x, $xs,*])
+--   | `(⋯)       => `(v[$x, $tail]) -- Unexpands to `[x, y, z, ⋯]` for `⋯ : List α`
+--   | _          => throw ()
+-- | _ => throw ()
 
 @[simp]
-theorem Vec.nil_singleton (v1 v2 : Vec T 0) : v1 = v2 := by
+theorem Vect.nil_singleton (v1 v2 : Vect 0 T) : v1 = v2 := by
   funext; case _ i =>
   cases i; case _ i p => cases p
 
-@[simp]
-theorem Vec.uncons_cons_cancel : uncons (h::t) = (h, t) := by
-  simp [uncons, drop]; case _ n =>
-  apply And.intro _ _
-  case _ =>
-    cases n <;> simp [cons]
-  case _ =>
-    funext; case _ i =>
-    cases i; case _ i p =>
-    cases i <;> simp [cons, Fin.pred]
+-- @[simp]
+-- theorem Vect.uncons_cons_cancel : uncons (h::t) = ⟨h, t⟩ := by
+--   simp [uncons];
+
+-- @[simp]
+-- theorem Vect.head_drop_cancel : ((v 0) :: (drop v)) = v := by
+--   funext; case _ i =>
+--   cases i; case _ i p =>
+--   cases i <;> simp [cons, drop]
+
+-- theorem Vect.cons_iff_uncons {t : Vect T n} : v = h::t <-> uncons v = ⟨h, t⟩ := by
+--   apply Iff.intro
+--   case _ => intro e; subst e; simp
+--   case _ =>
+--     intro e; simp [uncons] at e
+--     cases e; case _ e1 e2 =>
+--     subst e1; subst e2; simp
+
+
+-- def Vect.induction
+--   {motive : {n : Nat} -> Vect T n -> Sort u}
+--   (nc : motive Vect.nil)
+--   (cc : ∀ {n t} {v : Vect T n}, motive v -> motive (t::v))
+--   (v : Vect T n)
+--   : motive v
+-- := by
+--   induction n
+--   case _ => rw [nil_singleton v]; exact nc
+--   case _ n ih =>
+--     generalize zdef : uncons v = z at *
+--     rcases z with ⟨h, t⟩
+--     have lem := cons_iff_uncons.2 zdef
+--     rw [lem]; apply cc (ih t)
+
+
+-- -- theorem Vect.induction1
+-- --   {motive : Vect T 1 -> Prop}
+-- --   (h : ∀ {t : T}, motive v[t])
 
 @[simp]
-theorem Vec.head_drop_cancel : v 0 :: drop v = v := by
-  funext; case _ i =>
-  cases i; case _ i p =>
-  cases i <;> simp [cons, drop]
-
-theorem Vec.cons_iff_uncons {t : Vec T n} : v = h::t <-> uncons v = (h, t) := by
-  apply Iff.intro
-  case _ => intro e; subst e; simp
-  case _ =>
-    intro e; simp [uncons] at e
-    cases e; case _ e1 e2 =>
-    subst e1; subst e2; simp
-
-
-def Vec.induction
-  {motive : {n : Nat} -> Vec T n -> Sort u}
-  (nc : motive Vec.nil)
-  (cc : ∀ {n t} {v : Vec T n}, motive v -> motive (t::v))
-  (v : Vec T n)
-  : motive v
-:= by
-  induction n
-  case _ => rw [nil_singleton v]; exact nc
-  case _ n ih =>
-    generalize zdef : uncons v = z at *
-    rcases z with ⟨h, t⟩
-    have lem := cons_iff_uncons.2 zdef
-    rw [lem]; apply cc (ih t)
-
-
--- theorem Vec.induction1
---   {motive : Vec T 1 -> Prop}
---   (h : ∀ {t : T}, motive v[t])
-
-@[simp]
-instance : GetElem (Vec α n) (Fin n) α (λ _ _ => True) where
+instance : GetElem (Vect n α) (Fin n) α (λ _ _ => True) where
   getElem xs i _ := xs i
 
 @[simp]
-instance : GetElem? (Vec α n) (Fin n) α (λ _ _ => True) where
+instance : GetElem? (Vect n α) (Fin n) α (λ _ _ => True) where
   getElem? xs i := .some (xs i)
 
 @[simp]
-theorem get_cons_head {t : Vec T n} : (h::t) 0 = h := by simp [Vec.cons]
+theorem get_cons_head {t : Vect T n} : (h::t) 0 = h := by simp [Vect.cons]
 
 @[simp]
-theorem get_cons_tail_succ {t : Vec T n} : (h::t) (Fin.succ i) = t i := by
-  simp [Vec.cons]; intro h; cases h
+theorem get_cons_tail_succ {t : Vect T n} : (h::t) (Fin.succ i) = t i := by
+  simp [Vect.cons];
 
-@[simp]
-theorem get1_0 : v[a] 0 = a := by simp
+-- @[simp]
+-- theorem get1_0 : v[a] 0 = a := by simp
 
-@[simp]
-theorem get2_0 : v[a, b] 0 = a := by simp
+-- @[simp]
+-- theorem get2_0 : v[a, b] 0 = a := by simp
 
-@[simp]
-theorem get2_1 : v[a, b] 1 = b := by simp [Vec.cons]
+-- @[simp]
+-- theorem get2_1 : v[a, b] 1 = b := by simp [Vect.cons]
 
-def Vec.map (f : A -> B) (v : Vec A n) : Vec B n := λ i => f (v i)
+-- def Vect.map (f : A -> B) (v : Vect A n) : Vect B n := λ i => f (v i)
 
-@[simp]
-def Vec.map2 (v1 : Vec A n) (v2 : Vec B n) (f : A -> B -> C)  : Vec C n := λ i => f (v1 i) (v2 i)
+-- @[simp]
+-- def Vect.map2 (v1 : Vect A n) (v2 : Vect B n) (f : A -> B -> C)  : Vect C n := λ i => f (v1 i) (v2 i)
 
-@[simp]
-theorem Vec.map_nil : Vec.map f v[] = v[] := by
-  funext; case _ x => apply Fin.elim0 x
+-- @[simp]
+-- theorem Vect.map_nil : Vect.map f v[] = v[] := by
+--   funext; case _ x => apply Fin.elim0 x
 
-@[simp]
-theorem Vec.map_cons : Vec.map f (h::t) = (f h)::Vec.map f t := by
-  funext; case _ i =>
-  cases i using Fin.cases <;> simp [Vec.map]
+-- @[simp]
+-- theorem Vect.map_cons : Vect.map f (h::t) = (f h)::Vect.map f t := by
+--   funext; case _ i =>
+--   cases i using Fin.cases <;> simp [Vect.map]
 
-@[simp]
-theorem Vec.eta0 (t : Vec T 0) : t = v[] := by apply Vec.nil_singleton
+-- @[simp]
+-- theorem Vect.eta0 (t : Vect T 0) : t = v[] := by apply Vect.nil_singleton
 
-@[simp]
-theorem Vec.eta1 (t : Vec T 1) : v[t 0] = t := by
-  funext; case _ i =>
-  cases i using Fin.cases1; simp
+-- @[simp]
+-- theorem Vect.eta1 (t : Vect T 1) : v[t 0] = t := by
+--   funext; case _ i =>
+--   cases i using Fin.cases1; simp
 
-@[simp]
-theorem Vec.eta2 (t : Vec T 2) : v[t 0, t 1] = t := by
-  funext; case _ i =>
-  cases i using Fin.cases2 <;> simp
+-- @[simp]
+-- theorem Vect.eta2 (t : Vect T 2) : v[t 0, t 1] = t := by
+--   funext; case _ i =>
+--   cases i using Fin.cases2 <;> simp
 
-@[simp]
-theorem Vec.inv1 {a b : Vec T 1} : a = b <-> a 0 = b 0 := by
-  apply Iff.intro; intro h; subst h; rfl
-  intro h; funext; case _ i =>
-  cases i using Fin.cases1; exact h
+-- @[simp]
+-- theorem Vect.inv1 {a b : Vect T 1} : a = b <-> a 0 = b 0 := by
+--   apply Iff.intro; intro h; subst h; rfl
+--   intro h; funext; case _ i =>
+--   cases i using Fin.cases1; exact h
 
-@[simp]
-theorem Vec.inv2 {a b : Vec T 2} : a = b <-> a 0 = b 0 ∧ a 1 = b 1 := by
-  apply Iff.intro; intro h; subst h; simp
-  intro h; funext; case _ i =>
-  cases i using Fin.cases2 <;> simp [*]
+-- @[simp]
+-- theorem Vect.inv2 {a b : Vect T 2} : a = b <-> a 0 = b 0 ∧ a 1 = b 1 := by
+--   apply Iff.intro; intro h; subst h; simp
+--   intro h; funext; case _ i =>
+--   cases i using Fin.cases2 <;> simp [*]
 
-def Vec.update (i : Fin n) (t : T) (ts : Vec T n) : Vec T n
-| x => if i = x then t else ts x
+-- def Vect.update (i : Fin n) (t : T) (ts : Vect T n) : Vect T n
+-- | x => if i = x then t else ts x
 
-@[simp]
-theorem Vec.update_eq : update i t ts i = t := by simp [update]
+-- @[simp]
+-- theorem Vect.update_eq : update i t ts i = t := by simp [update]
 
-theorem Vec.update_neq : ∀ j ≠ i, update i t ts j = ts j := by
-  simp [update]; intro j h1 h2
-  exfalso; apply h1; rw [h2]
+-- theorem Vect.update_neq : ∀ j ≠ i, update i t ts j = ts j := by
+--   simp [update]; intro j h1 h2
+--   exfalso; apply h1; rw [h2]
 
-theorem Vec.update_stable i t {ts ts' : Vec T n} :
-  (∀ j ≠ i, ts j = ts' j) ->
-  ∀ j ≠ i, ts j = update i t ts' j
-:= by
-  intro h1 j h2; simp [update, *]
-  intro h3; exfalso; apply h2; rw [h3]
+-- theorem Vect.update_stable i t {ts ts' : Vect T n} :
+--   (∀ j ≠ i, ts j = ts' j) ->
+--   ∀ j ≠ i, ts j = update i t ts' j
+-- := by
+--   intro h1 j h2; simp [update, *]
+--   intro h3; exfalso; apply h2; rw [h3]
 
--- def Vec.fold (acc : A -> B -> B) (d : B) : Vec A n -> B :=
---   Vec.induction (motive := λ _ => B) d (@fun _ hd _ ih => acc hd ih)
+-- -- def Vect.fold (acc : A -> B -> B) (d : B) : Vect A n -> B :=
+-- --   Vect.induction (motive := λ _ => B) d (@fun _ hd _ ih => acc hd ih)
 
-def Vec.fold (acc : A -> B -> B) (d : B) : {n : Nat} -> Vec A n -> B
-| 0, _ => d
-| _ + 1, vs =>
-  let (h, tl) := uncons vs
-  acc h (fold acc d tl)
+-- def Vect.fold (acc : A -> B -> B) (d : B) : {n : Nat} -> Vect A n -> B
+-- | 0, _ => d
+-- | _ + 1, vs =>
+--   let (h, tl) := uncons vs
+--   acc h (fold acc d tl)
 
 
-@[simp]
-theorem Vec.fold_nil : fold acc d Vec.nil = d := by simp [fold]
+-- @[simp]
+-- theorem Vect.fold_nil : fold acc d Vect.nil = d := by simp [fold]
 
-@[simp]
-theorem Vec.fold_cons : fold acc d (hd :: tl) = acc hd (fold acc d tl) := by simp [fold]
+-- @[simp]
+-- theorem Vect.fold_cons : fold acc d (hd :: tl) = acc hd (fold acc d tl) := by simp [fold]
 
-def Vec.length (_ : Vec A n) : Nat := n
+-- def Vect.length (_ : Vect A n) : Nat := n
 
-theorem Vec.length_bound : (v : Vec A n) -> v.length == n := by
-  intro v
-  unfold Vec.length
-  induction n <;> (simp at *)
+-- theorem Vect.length_bound : (v : Vect A n) -> v.length == n := by
+--   intro v
+--   unfold Vect.length
+--   induction n <;> (simp at *)
 
-def Vec.fold2 (acc : A -> B -> C -> C) (d : C) : {n1 n2 : Nat} -> (n1 = n2) -> Vec A n1 -> Vec B n2 -> C
-| 0, 0, rfl, _, _ => d
-| _ + 1, _ + 1, h, va, vb =>
-  let (h1, tl1) := uncons va
-  let (h2, tl2) := uncons vb
-  acc h1 h2 (fold2 acc d (by cases h; rfl) tl1 tl2)
+-- def Vect.fold2 (acc : A -> B -> C -> C) (d : C) : {n1 n2 : Nat} -> (n1 = n2) -> Vect A n1 -> Vect B n2 -> C
+-- | 0, 0, rfl, _, _ => d
+-- | _ + 1, _ + 1, h, va, vb =>
+--   let (h1, tl1) := uncons va
+--   let (h2, tl2) := uncons vb
+--   acc h1 h2 (fold2 acc d (by cases h; rfl) tl1 tl2)
 
-@[simp]
-def Vec.sum : {n : Nat} -> Vec Nat n -> Nat
-| 0, _ => 0
-| _ + 1, ts => ts 0 + ts.drop.sum
+-- @[simp]
+-- def Vect.sum : {n : Nat} -> Vect Nat n -> Nat
+-- | 0, _ => 0
+-- | _ + 1, ts => ts 0 + ts.drop.sum
 
-@[simp]
-def Vec.beq (beq : T -> T -> Bool) : {n1 n2 : Nat} -> (n1 = n2) -> Vec T n1 -> Vec T n2 -> Bool
-| 0, 0, rfl, _, _ => true
-| _ + 1, _ + 1, h, v1, v2 =>
-  let (h1, t1) := Vec.uncons v1
-  let (h2, t2) := Vec.uncons v2
-  beq h1 h2 && Vec.beq beq (by cases h; rfl) t1 t2
+-- @[simp]
+-- def Vect.beq (beq : T -> T -> Bool) : {n1 n2 : Nat} -> (n1 = n2) -> Vect T n1 -> Vect T n2 -> Bool
+-- | 0, 0, rfl, _, _ => true
+-- | _ + 1, _ + 1, h, v1, v2 =>
+--   let (h1, t1) := Vect.uncons v1
+--   let (h2, t2) := Vect.uncons v2
+--   beq h1 h2 && Vect.beq beq (by cases h; rfl) t1 t2
 
-instance instBEq_Vec [BEq T] : BEq (Vec T n) where
-  beq := Vec.beq BEq.beq rfl
+-- instance instBEq_Vect [BEq T] : BEq (Vect T n) where
+--   beq := Vect.beq BEq.beq rfl
 
-def Vec.rfl [BEq T] [ReflBEq T] : ∀ {v : Vec T n}, (v == v) = true := by
-intro v
-match n, v with
-| 0, v => simp [instBEq_Vec] at *
-| n + 1, v =>
-    simp [instBEq_Vec] at *
-    let (x, v') := v.uncons
-    simp at *; apply @Vec.rfl _ n _ _ v'
+-- def Vect.rfl [BEq T] [ReflBEq T] : ∀ {v : Vect T n}, (v == v) = true := by
+-- intro v
+-- match n, v with
+-- | 0, v => simp [instBEq_Vect] at *
+-- | n + 1, v =>
+--     simp [instBEq_Vect] at *
+--     let (x, v') := v.uncons
+--     simp at *; apply @Vect.rfl _ n _ _ v'
 
-instance instReflBEq_Vec [BEq T] [ReflBEq T] : ReflBEq (Vec T n) where
-  rfl := Vec.rfl
+-- instance instReflBEq_Vect [BEq T] [ReflBEq T] : ReflBEq (Vect T n) where
+--   rfl := Vect.rfl
 
 
 variable {S T : Type} [RenMap T] [SubstMap S T]
 
-@[simp]
-theorem Vec.subst_cons {t : Vec S n} {σ : Subst T}
-  : ((h::t) i)[σ:T] = (h[σ:_]::map (·[σ:_]) t) i
-:= by
-  induction i using Fin.induction <;> simp at *
-  case _ i ih =>
-    cases n; apply Fin.elim0 i
-    case _ n =>
-    cases i using Fin.cases <;> simp [Vec.map] at *
+-- @[simp]
+-- theorem Vect.subst_cons {t : Vect S n} {σ : Subst T}
+--   : ((h::t) i)[σ:T] = (h[σ:_]::map (·[σ:_]) t) i
+-- := by
+--   induction i using Fin.induction <;> simp at *
+--   case _ i ih =>
+--     cases n; apply Fin.elim0 i
+--     case _ n =>
+--     cases i using Fin.cases <;> simp [Vect.map] at *
 
 omit [RenMap T] [SubstMap S T] in
-def Vec.indexOf [BEq Q] (c : Q) {n : Nat} (v :  Vec Q n) : Option (Fin n) :=
+def Vect.indexOf [BEq Q] (c : Q) {n : Nat} (v :  Vect n Q) : Option (Fin n) :=
 match n with
 | 0 => none
 | n + 1 =>
-    let (found, i, _) := Vec.fold (λ x (found, found_idx, i) =>
+    let (found, i, _) := Vect.fold (false, 0, 0) (λ x (found, found_idx, i) =>
       if not found
         then if x == c
                 then (true, i, i + 1)
                 else (found, found_idx, i + 1)
         else (found, found_idx, i + 1)
-    ) (false, 0, 0) v
+    )  v
     if found then return Fin.ofNat (n + 1) (n - i) else none
 
-def Vec.indexOf_aux [BEq Q][LawfulBEq Q] (c : Q) (n : Nat) : Nat -> (Vec Q n) -> Option Nat := λ i v =>
+def Vect.indexOf_aux [BEq Q][LawfulBEq Q] (c : Q) (n : Nat) : Nat -> (Vect n Q) -> Option Nat := λ i v =>
 match n, v with
 | 0, _ => none
 | n + 1, v' =>
     match v'.uncons with
-    | (x, v') => if x == c
+    | ⟨x, v'⟩ => if x == c
       then i
-      else (Vec.indexOf_aux c n (i + 1) v')
+      else (Vect.indexOf_aux c n (i + 1) v')
 
-def Vec.indexOf' [BEq Q][LawfulBEq Q] (c : Q) (v : Vec Q n) : Option (Fin n) :=
+def Vect.indexOf' [BEq Q][LawfulBEq Q] (c : Q) (v : Vect n Q) : Option (Fin n) :=
 match n with
 | 0 => none
-| n + 1 => (Vec.indexOf_aux c (n + 1) 0 v).map (Fin.ofNat (n + 1))
+| n + 1 => (Vect.indexOf_aux c (n + 1) 0 v).map (Fin.ofNat (n + 1))
 
 
-#guard Vec.indexOf "x" v["x", "y", "p"] == some 0
-#guard Vec.indexOf "y" v["x", "y", "p"] == some 1
-#guard Vec.indexOf "p" v["x", "y", "p"] == some 2
-#guard Vec.indexOf "z" v["x", "y", "p"] == none
+#guard Vect.indexOf "x" (["x", "y", "p"] : Vect 3 String) == some 0
+#guard Vect.indexOf "y" (["x", "y", "p"] : Vect 3 String) == some 1
+#guard Vect.indexOf "p" (["x", "y", "p"] : Vect 3 String) == some 2
+#guard Vect.indexOf "z" (["x", "y", "p"] : Vect 3 String) == none
 
-#guard Vec.indexOf' "x" v["x", "y", "p"] == some 0
-#guard Vec.indexOf' "y" v["x", "y", "p"] == some 1
-#guard Vec.indexOf' "p" v["x", "y", "p"] == some 2
-#guard Vec.indexOf' "z" v["x", "y", "p"] == none
+#guard Vect.indexOf' "x" (["x", "y", "p"] : Vect 3 String) == some 0
+#guard Vect.indexOf' "y" (["x", "y", "p"] : Vect 3 String) == some 1
+#guard Vect.indexOf' "p" (["x", "y", "p"] : Vect 3 String) == some 2
+#guard Vect.indexOf' "z" (["x", "y", "p"] : Vect 3 String) == none
 
-def Vec.HasUniqueElems [BEq Q] (v : Vec Q n) := ∀ i j, i ≠ j -> (v i) ≠ (v j)
+def Vect.HasUniqueElems [BEq Q] (v : Vect n Q) := ∀ i j, i ≠ j -> (v i) ≠ (v j)
 
 
-theorem Vec.indexOf_correct [BEq Q] {v : Vec Q n} :
+theorem Vect.indexOf_correct [BEq Q] {v : Vect n Q} :
   v.indexOf x = some i ->
   (v i) = x := by
 intro h
 induction n <;> simp at *
 case _ =>  cases i; simp [indexOf] at h
-case _ n ih =>
-  match v.uncons with
-  | (_, v') =>
-    sorry
+case _ n ih => sorry
 
-theorem Vec.indexOf'_le [BEq Q] [LawfulBEq Q] {v : Vec Q n} :
+theorem Vect.indexOf'_le [BEq Q] [LawfulBEq Q] {v : Vect n Q} :
   v.indexOf' x = some i ->
   i < n := by
 intro h
 induction n <;> simp at *
 case _ => cases i; simp [indexOf'] at h
 
-theorem Vec.indexOf'_aux_le [BEq Q] [LawfulBEq Q] {v : Vec Q n} :
+theorem Vect.indexOf'_aux_le [BEq Q] [LawfulBEq Q] {v : Vect n Q} :
   v.indexOf_aux x n 0 = some i ->
   i < n := by
 intro j
 induction n generalizing i
-case _ => unfold Vec.indexOf_aux at j; cases j
+case _ => unfold Vect.indexOf_aux at j; cases j
 case _ ih =>
-  unfold Vec.indexOf_aux at j;
+  unfold Vect.indexOf_aux at j;
   split at j; simp at j;
   sorry
 
 
 
-theorem Vec.indexOf'_correct [BEq Q] [LawfulBEq Q] {v : Vec Q n} :
+theorem Vect.indexOf'_correct [BEq Q] [LawfulBEq Q] {v : Vect n Q} :
   v.indexOf' x = some i ->
   v i = x := by
 intro j; induction n
 case _ => simp [indexOf'] at j
 case _ n ih => sorry
-  -- have lem := Vec.indexOf'_le j
+  -- have lem := Vect.indexOf'_le j
   -- simp [indexOf', indexOf_aux] at *; rcases j with ⟨n, j1, j2⟩
   -- have ih' := ih (i := i + 1) (v := v.uncons.snd)
   -- split at j1
@@ -375,7 +333,7 @@ case _ n ih => sorry
 
 
 
-def Vec.seq_lemma (vs : Vec (Option Q) n) :
+def Vect.seq_lemma (vs : Vect (Option Q) n) :
   (Σ' (i : Fin n), (vs i).isSome = false) ⊕ ((i : Fin n) -> Σ' A, (vs i) = some A)
 := by {
     induction n
@@ -404,7 +362,7 @@ def Vec.seq_lemma (vs : Vec (Option Q) n) :
           case _ i => rw [lem]; simp; apply ih i
   }
 
-def Vec.seq (vs : Vec (Option Q) n) : Option (Vec Q n) :=
+def Vect.seq (vs : Vect (Option Q) n) : Option (Vect Q n) :=
   match seq_lemma vs with
   | .inl h => none
   | .inr h => some (λ i => Option.get (vs i) (by {
@@ -413,17 +371,17 @@ def Vec.seq (vs : Vec (Option Q) n) : Option (Vec Q n) :=
     rw [e]; simp
   }))
 
-theorem Vec.seq_sound {vs : Vec (Option Q) n} {vs' : Vec Q n}:
+theorem Vect.seq_sound {vs : Vect (Option Q) n} {vs' : Vect Q n}:
   vs.seq = some vs' ->
   ∀ i, (vs i) = some (vs' i) := by
 intro h i
--- simp [Vec.seq, Vec.seq_lemma] at h
+-- simp [Vect.seq, Vect.seq_lemma] at h
 match n with
 | 0 => simp at *; cases i; omega
 | n + 1 =>
   apply @Fin.inductionOn n i
   case _ =>
-    simp [Vec.seq, Vec.seq_lemma] at h; split at h <;> simp at *
+    simp [Vect.seq, Vect.seq_lemma] at h; split at h <;> simp at *
     case _ x h' heq =>
       cases x
       case _ =>
@@ -438,7 +396,7 @@ match n with
 
 
 -- Returns the 1st element if all the elements are equal
-def Vec.get_elem_if_eq [BEq Q] (vs : Vec Q n) : Option Q :=
+def Vect.get_elem_if_eq [BEq Q] (vs : Vect Q n) : Option Q :=
 match n with
 | 0 => none
 | _ + 1 =>  match vs.uncons with
@@ -446,11 +404,11 @@ match n with
     if vs'.fold (λ c acc => c == h && acc) true
     then return h else none
 
-theorem Vec.get_elem_if_eq_sound [BEq Q] {vs : Vec Q n} {t : Q} :
+theorem Vect.get_elem_if_eq_sound [BEq Q] {vs : Vect Q n} {t : Q} :
   vs.get_elem_if_eq = some t ->
   ∀ i, vs i = t := by
 intro h i
-induction n <;> simp [Vec.get_elem_if_eq, Vec.uncons] at *
+induction n <;> simp [Vect.get_elem_if_eq, Vect.uncons] at *
 case _ n ih =>
   replace ih := @ih vs.drop
   split at ih <;> simp at *
@@ -459,20 +417,20 @@ case _ n ih =>
 
 
 
-def Vec.elems_eq_to [BEq Q] (e : Q) : {n : Nat} -> (vs : Vec Q n) -> Bool
+def Vect.elems_eq_to [BEq Q] (e : Q) : {n : Nat} -> (vs : Vect Q n) -> Bool
 | 0, _ => true
 | _ + 1, vs =>
   match vs.uncons with
   | (h, vs') =>
     if h == e then vs'.elems_eq_to e else false
 
-theorem Vec.elems_eq_to_sound [BEq Q] {e : Q} {vs : Vec Q n} :
+theorem Vect.elems_eq_to_sound [BEq Q] {e : Q} {vs : Vect Q n} :
   vs.elems_eq_to e = true ->
   ∀ i, (vs i) = e := by sorry
 
-theorem vec_size_1 [BEq Q]: Vec Q (0 + 1) = Vec Q 1 := by simp
+theorem vec_size_1 [BEq Q]: Vect Q (0 + 1) = Vect Q 1 := by simp
 
-theorem Vec.uncons_injective [BEq Q] : Function.Injective (α := Vec Q (n + 1)) (β := Q × Vec Q n) Vec.uncons := by
+theorem Vect.uncons_injective [BEq Q] : Function.Injective (α := Vect Q (n + 1)) (β := Q × Vect Q n) Vect.uncons := by
 intro v1 v2; induction n
 sorry
 sorry
